case_studies/refinedrust-20-paper-examples/output/real_refinedrust_paper_examples/proofs/proof_REFaListTasstd_iter_IntoIterator_into_iter.v
@@ -1,0 +1,22 @@
+From caesium Require Import lang notation.
+From refinedrust Require Import typing shims.
+From refinedrust.examples.real_refinedrust_paper_examples.generated Require Import generated_code_real_refinedrust_paper_examples generated_specs_real_refinedrust_paper_examples generated_template_REFaListTasstd_iter_IntoIterator_into_iter.
+
+Set Default Proof Using "Type".
+
+Section proof.
+Context `{RRGS : !refinedrustGS Σ}.
+
+Lemma REFaListTasstd_iter_IntoIterator_into_iter_proof (π : thread_id) :
+  REFaListTasstd_iter_IntoIterator_into_iter_lemma π.
+Proof.
+  REFaListTasstd_iter_IntoIterator_into_iter_prelude.
+
+  rep <-! liRStep; liShow.
+
+  all: print_remaining_goal.
+  Unshelve. all: sidecond_solver.
+  Unshelve. all: sidecond_hammer.
+  Unshelve. all: print_remaining_sidecond.
+Qed.
+End proof.
