case_studies/refinedrust-20-paper-examples/output/real_refinedrust_paper_examples/proofs/trait_incl_REFaListTasstd_iter_IntoIterator_spec_subsumption_correct.v
@@ -1,0 +1,21 @@
+From caesium Require Import lang notation.
+From refinedrust Require Import typing shims.
+From refinedrust.examples.real_refinedrust_paper_examples.generated Require Import generated_specs_real_refinedrust_paper_examples.
+
+Set Default Proof Using "Type".
+
+Section proof.
+Context `{RRGS : !refinedrustGS Σ}.
+
+Lemma REFaListTasstd_iter_IntoIterator_spec_subsumption_correct  : (REFaListTasstd_iter_IntoIterator_spec_subsumption).
+Proof.
+  unfold REFaListTasstd_iter_IntoIterator_spec_subsumption; solve_trait_incl_prelude.
+  all: repeat liRStep; liShow.
+  all: print_remaining_trait_goal.
+  Unshelve.
+  all: sidecond_solver.
+  Unshelve.
+  all: sidecond_hammer.
+Qed.
+
+End proof.
