hinata_mikami/linkedlist/output/linkedlist/generated/generated_template_Heap_alloc.v
@@ -25,13 +25,13 @@ Set Default Proof Using "Type".
 
 Section proof.
 Context `{RRGS : !refinedrustGS Σ}.
-Definition LinkedList_alloc_lemma (π : thread_id) : Prop :=
+Definition Heap_alloc_lemma (π : thread_id) : Prop :=
   ∀ (Box_T_into_raw_Node_loc : loc) (Box_T_new_Node_loc : loc) (Vec_TA_push_mutNode_std_alloc_Global_loc : loc) (ptr_null_mut_Node_loc : loc) , 
   syn_type_is_layoutable (((Box_sls (Node_st) ((Global_sls : syn_type))) : syn_type)) →
   syn_type_is_layoutable ((Global_sls : syn_type)) →
   syn_type_is_layoutable (((Vec_sls (PtrSynType) ((Global_sls : syn_type))) : syn_type)) →
+  syn_type_is_layoutable ((Heap_sls : syn_type)) →
   syn_type_is_layoutable ((Node_sls : syn_type)) →
-  syn_type_is_layoutable ((LinkedList_sls : syn_type)) →
   Box_T_into_raw_Node_loc ◁ᵥ{π, MetaNone} Box_T_into_raw_Node_loc @ function_ptr [((Box_sls (Node_st) ((Global_sls : syn_type))) : syn_type)] (<tag_type> spec! ( *[]) : 0 | ( *[]) : ([] : list RT), fn_spec_add_late_pre (type_of_Box_T_into_raw (RRGS:=RRGS) ((Node_inv_t_rt)) (Node_st)  <TY> (Node_inv_t    <INST!>) <INST!>) (λ π, (True)
   ∗ (⌜(trait_incl_of_Box_T_into_raw ((Node_inv_t_rt)) (Node_st)  <TY> (Node_inv_t    <INST!>) <INST!>)%Z⌝))%I) -∗
   Box_T_new_Node_loc ◁ᵥ{π, MetaNone} Box_T_new_Node_loc @ function_ptr [Node_st] (<tag_type> spec! ( *[]) : 0 | ( *[]) : ([] : list RT), fn_spec_add_late_pre (type_of_Box_T_new (RRGS:=RRGS) ((Node_inv_t_rt)) (Node_st)  <TY> (Node_inv_t    <INST!>) <INST!>) (λ π, (True)
@@ -40,20 +40,20 @@ Definition LinkedList_alloc_lemma (π : thread_id) : Prop :=
   ∗ (⌜(trait_incl_of_Vec_TA_push (loc) ((((Global_rt)))) (PtrSynType) ((Global_sls : syn_type)) GlobalasAllocator_spec_attrs (spec! ( *[]) : 0 | ( *[]) : ([] : list RT), GlobalasAllocator_spec   <INST!>)  <TY> alias_ptr_t <TY> (Global_ty   <INST!>) <LFT> late_lft_0 <INST!>)%Z⌝))%I) -∗
   ptr_null_mut_Node_loc ◁ᵥ{π, MetaNone} ptr_null_mut_Node_loc @ function_ptr [] (<tag_type> spec! ( *[]) : 0 | ( *[]) : ([] : list RT), fn_spec_add_late_pre (type_of_ptr_null_mut (RRGS:=RRGS) ((Node_inv_t_rt)) (Node_st)  <TY> (Node_inv_t    <INST!>) <INST!>) (λ π, (True)
   ∗ (⌜(trait_incl_of_ptr_null_mut ((Node_inv_t_rt)) (Node_st)  <TY> (Node_inv_t    <INST!>) <INST!>)%Z⌝))%I) -∗
-  typed_function π (LinkedList_alloc_def Box_T_into_raw_Node_loc  Box_T_new_Node_loc  Vec_TA_push_mutNode_std_alloc_Global_loc  ptr_null_mut_Node_loc  ) (<tag_type> spec! ( *[ulft_1]) : 1 | ( *[]) : ([] : list RT), fn_spec_add_late_pre (type_of_LinkedList_alloc  <LFT> ulft_1 <INST!>) (λ π, (True)
-  ∗ (⌜(trait_incl_of_LinkedList_alloc <LFT> ulft_1 <INST!>)%Z⌝))).
+  typed_function π (Heap_alloc_def Box_T_into_raw_Node_loc  Box_T_new_Node_loc  Vec_TA_push_mutNode_std_alloc_Global_loc  ptr_null_mut_Node_loc  ) (<tag_type> spec! ( *[ulft_1]) : 1 | ( *[]) : ([] : list RT), fn_spec_add_late_pre (type_of_Heap_alloc  <LFT> ulft_1 <INST!>) (λ π, (True)
+  ∗ (⌜(trait_incl_of_Heap_alloc <LFT> ulft_1 <INST!>)%Z⌝))).
 End proof.
 
-Ltac LinkedList_alloc_prelude :=
-  unfold LinkedList_alloc_lemma;
-  set (FN_NAME := FUNCTION_NAME "LinkedList_alloc");
+Ltac Heap_alloc_prelude :=
+  unfold Heap_alloc_lemma;
+  set (FN_NAME := FUNCTION_NAME "Heap_alloc");
   intros;
   iStartProof;
   let ϝ := fresh "ϝ" in
   let ulft_1 := fresh "ulft_1" in
   let l := fresh "l" in
   let v := fresh "v" in
-  start_function "LinkedList_alloc" ϝ ( [ulft_1 [] ] ) ( [] ) ( [  l v ] ) (  l v );
+  start_function "Heap_alloc" ϝ ( [ulft_1 [] ] ) ( [] ) ( [  l v ] ) (  l v );
   intros arg_self arg_value;
   let π := get_π in
   let Σ := get_Σ in
